moving to github 2

BALFI_logic.thy
@@ -1,7 +1,7 @@
 theory BALFI_logic
   imports BA_logic
 begin
-nitpick_params[assms=true, user_axioms=true, show_all, expect=genuine, format=3] (*default Nitpick settings*)
+nitpick_params[assms=true, user_axioms=true, show_all, expect=genuine, format=3, timeout=60] (*default Nitpick settings*)
 
 (**The LFIs are a family of paraconsistent logics featuring a paraconsistent negation \<^bold>\<not>
 and a consistency operator \<^bold>\<circ> that can be used to recover some classical properties
@@ -15,17 +15,6 @@ axiomatization where
           LEM:  "a \<^bold>\<or> \<^bold>\<not>a \<^bold>\<approx> \<^bold>\<top>" and
           CONS: "a \<^bold>\<and> \<^bold>\<not>a \<^bold>\<and> \<^bold>\<circ>a \<^bold>\<approx> \<^bold>\<bottom>"
 
-
-(**This negation is of course boldly paraconsistent.*)
-lemma "[a, \<^bold>\<not>a \<^bold>\<turnstile> b]" nitpick oops (*countermodel*)
-lemma "[a, \<^bold>\<not>a \<^bold>\<turnstile> \<^bold>\<not>b]" nitpick oops (*countermodel*)
-lemma "[a, \<^bold>\<not>a \<^bold>\<turnstile>\<^sub>g b]" nitpick oops (*countermodel*) 
-lemma "[a, \<^bold>\<not>a \<^bold>\<turnstile>\<^sub>g \<^bold>\<not>b]" nitpick oops (*countermodel*)
-
-(**We can recover explosion using \<^bold>\<circ> (cf. 'principle of gentle explosion')*)
-lemma "[a, \<^bold>\<not>a, \<^bold>\<circ>a \<^bold>\<turnstile> b]" by (simp add: CONS bottom_def)
-
-
 (**The following axioms are commonly employed in the literature on LFIs to obtain stronger logics.
 We explore under which conditions they can be assumed while keeping the logic boldly paraconsistent.*)
 abbreviation ciw where "ciw \<equiv> \<forall>a. [\<^bold>\<turnstile> \<^bold>\<circ>a \<^bold>\<or> (a \<^bold>\<and> \<^bold>\<not>a)]"
@@ -38,7 +27,7 @@ abbreviation ca_disj where "ca_disj \<equiv> \<forall>a b. [\<^bold>\<turnstile>
 abbreviation ca_impl where "ca_impl \<equiv> \<forall>a b. [\<^bold>\<turnstile> (\<^bold>\<circ>a \<^bold>\<and> \<^bold>\<circ>b) \<^bold>\<rightarrow> \<^bold>\<circ>(a \<^bold>\<rightarrow> b)]"
 abbreviation ca where "ca \<equiv> ca_conj \<and> ca_disj \<and> ca_impl"
 
-lemma "ciw \<longleftrightarrow> (\<forall>a. \<^bold>\<circ>a \<^bold>\<approx> \<^bold>\<midarrow>(a \<^bold>\<and> \<^bold>\<not>a))" by (metis CONS compl_def join_def meet_def)
+lemma "ciw \<longleftrightarrow> (\<forall>a. \<^bold>\<circ>a \<^bold>\<approx> \<^bold>\<sim>(a \<^bold>\<and> \<^bold>\<not>a))" by (metis CONS compl_def join_def meet_def)
 lemma "ci \<longleftrightarrow> (\<forall>a. \<^bold>\<not>\<^bold>\<circ>a \<^bold>\<approx> a \<^bold>\<and> \<^bold>\<not>a)" by (metis CONS LEM impl_def join_def meet_def)
 lemma "cl \<longleftrightarrow> (\<forall>a. \<^bold>\<circ>a \<^bold>\<approx> \<^bold>\<not>(a \<^bold>\<and> \<^bold>\<not>a))" by (metis CONS LEM impl_def join_def meet_def)
 lemma "cf \<longleftrightarrow> (\<forall>a. a \<^bold>\<and> \<^bold>\<not>\<^bold>\<not>a \<^bold>\<approx> \<^bold>\<not>\<^bold>\<not>a)" by (metis impl_def meet_def)
@@ -47,8 +36,43 @@ lemma "ca_conj \<longleftrightarrow> (\<forall>a b. (\<^bold>\<circ>a \<^bold>\<
 lemma "ca_disj \<longleftrightarrow> (\<forall>a b. (\<^bold>\<circ>a \<^bold>\<and> \<^bold>\<circ>b) \<^bold>\<and> \<^bold>\<circ>(a \<^bold>\<or> b) \<^bold>\<approx> \<^bold>\<circ>a \<^bold>\<and> \<^bold>\<circ>b)" by (metis impl_def meet_def)
 lemma "ca_impl \<longleftrightarrow> (\<forall>a b. (\<^bold>\<circ>a \<^bold>\<and> \<^bold>\<circ>b) \<^bold>\<and> \<^bold>\<circ>(a \<^bold>\<rightarrow> b) \<^bold>\<approx> \<^bold>\<circ>a \<^bold>\<and> \<^bold>\<circ>b)" by (metis impl_def meet_def)
 
-lemma "cl \<and> ce \<longrightarrow> (\<forall>a. [a \<^bold>\<turnstile> \<^bold>\<circ>a])" using CONS oops (*TODO*)
 
+(**The principle of 'explosion' or ex contradictione (sequitur) quodlibet.*)
+abbreviation "ECQ  \<equiv> \<forall>a b. [a, \<^bold>\<not>a \<^bold>\<turnstile> b]"
+abbreviation "ECQg \<equiv> \<forall>a b. [a, \<^bold>\<not>a \<^bold>\<turnstile>\<^sub>g b]"
+(**The property below is a weaker variant of 'explosion'.
+Logics with a negation satisfying this property are sometimes called "boldly paraconsistent".*)
+abbreviation "wECQ  \<equiv> \<forall>a b. [a, \<^bold>\<not>a \<^bold>\<turnstile> \<^bold>\<not>b]"
+abbreviation "wECQg \<equiv> \<forall>a b. [a, \<^bold>\<not>a \<^bold>\<turnstile>\<^sub>g \<^bold>\<not>b]"
 
-lemma "cl \<and> ci" nitpick[satisfy] oops (*TODO*)
+lemma "ECQ \<longrightarrow> ECQg" by (metis meet_def)
+lemma "ECQg \<longrightarrow> ECQ" nitpick oops (*counterexample found*)
+lemma "ECQ \<longrightarrow> wECQ" by auto
+lemma "wECQ \<longrightarrow> ECQ" nitpick oops (*counterexample found*)
+lemma "ECQg \<longrightarrow> wECQg" by auto
+lemma "wECQg \<longrightarrow> ECQg" nitpick oops (*counterexample found*)
+
+(**The LFI negation as defined above is (boldly) paraconsistent in all accounts.*)
+lemma "ECQ" nitpick oops (*countermodel*)
+lemma "ECQg" nitpick oops (*countermodel*)
+lemma "wECQ" nitpick oops (*countermodel*) 
+lemma "wECQg" nitpick oops (*countermodel*)
+
+(**We can recover explosion using \<^bold>\<circ> (cf. 'principle of gentle explosion')*)
+lemma "[a, \<^bold>\<not>a, \<^bold>\<circ>a \<^bold>\<turnstile> b]" by (simp add: CONS bottom_def)
+
+(**We can employ model finder Nitpick to generate models (option: satisfy) of a given cardinality
+(option: card w=2, i.e. 4-valued powerset algebras).
+We ask Nitpick to generate up to 100 models (Nitpick technical disclaimer: some models may be duplicated).*)
+lemma True nitpick[satisfy, card w=2, max_genuine=100] oops
+
+(**We can employ Nitpick to generate (boldly) paraconsistent models satisfying different conditions.
+For instance, we can find models satisfying cf, cf & ci, and cl but not cf, respectively.*)
+lemma "\<not>wECQ \<and> cf" nitpick[satisfy, card w=2, max_genuine=10] oops
+lemma "\<not>wECQ \<and> cf \<and> ci" nitpick[satisfy, card w=4, max_genuine=10] oops
+lemma "\<not>wECQ \<and> cl \<and> \<not>cf" nitpick[satisfy, card w=2, max_genuine=10] oops (*only 2 are returned!*)
+
+(**Observe, that Nitpick cannot find models with smaller cardinalities than the ones shown above.
+Also note that Nitpick might find different models each time it runs.*)
+
 end
