NM_logic.thy
@@ -7,5 +7,7 @@ nitpick_params[assms=true, user_axioms=true, show_all, expect=genuine, format=3]
 (**Neighbourhood semantics for LFIs*)
 
 
+(* lemma "cl \<and> ce \<longrightarrow> (\<forall>a. [a \<^bold>\<turnstile> \<^bold>\<circ>a])" using CONS oops (*TODO*) *)
+(* lemma "cf \<and> ci \<longrightarrow> cl" using LEM CONS oops (*TODO*) *)
 
 end
